k-way merge progress

theories/ert_logic/examples/kway_merge.v
@@ -4,25 +4,33 @@ From clutch.ert_logic Require Export problang_wp proofmode derived_laws ert_rule
 From clutch.ert_logic.examples Require Import lib.list min_heap_spec.
 Set Default Proof Using "Type*".
 
-Global Instance : Trichotomy (strict Z.le).
+(** * A [≤] head comparator for lists of intergers *)
+Definition list_Z_le : relation (list Z) :=
+  λ zs1 zs2,
+    match zs1, zs2 with
+    | [], _ => True
+    | _, [] => False
+    | z1 :: _, z2 :: _ => (z1 ≤ z2)%Z
+    end.
+
+Global Instance : RelDecision list_Z_le.
+Proof. intros [] []; firstorder. simpl. apply _. Qed.
+
+Global Instance : PreOrder list_Z_le.
 Proof.
-  intros ??.
-  destruct (decide (x = y)); [firstorder|].
-  destruct (decide (Z.le x y)).
-  - left. split; lia.
-  - right; right. split; lia.
+  constructor.
+  - intros []; by simpl.
+  - intros [] [] []; firstorder.
+    simpl in *. by etrans.
 Qed.
 
-Global Instance : TotalOrder Z.le. Proof. constructor; apply _. Qed.
-
-(** * A [≤] head comparator for lists of intergers *)
 Definition cmp_Z_list : val :=
   λ: "zs1" "zs2",
     let: "h1" := list_head "zs1" in
-    let: "h2" := list_head "zs2" in
     match: "h1" with
     | NONE => #true
     | SOME "z1" =>
+        let: "h2" := list_head "zs2" in
         match: "h2" with
         | NONE => #false
         | SOME "z2" => "z1" ≤ "z2"
@@ -32,31 +40,36 @@ Definition cmp_Z_list : val :=
 Section Z_comparator_spec.
   Context `{!ert_clutchGS Σ CostTick}.
 
-  Definition is_Z_list (z : Z) (v : val) : iProp Σ := ∃ zs, ⌜is_list (z :: zs) v⌝.
+  Definition is_Z_list (zs : list Z) (v : val) : iProp Σ := ⌜is_list zs v⌝.
 
-  Lemma wp_cmp_Z_list z1 z2 v1 v2 :
-    {{{ is_Z_list z1 v1 ∗ is_Z_list z2 v2 }}}
+  Lemma wp_cmp_Z_list zs1 zs2 v1 v2 :
+    {{{ is_Z_list zs1 v1 ∗ is_Z_list zs2 v2 }}}
       cmp_Z_list v1 v2
-    {{{ RET #(bool_decide (z1 ≤ z2)); is_Z_list z1 v1 ∗ is_Z_list z2 v2 }}}.
+    {{{ RET #(bool_decide (list_Z_le zs1 zs2)); is_Z_list zs1 v1 ∗ is_Z_list zs2 v2 }}}.
   Proof.
-    iIntros (?) "[[%zs1 %H1] [%zs2 %H2]] H".
+    iIntros (?) "[%Hzs1 %Hzs2] H".
     wp_rec. wp_pures.
-    wp_apply (wp_list_head _ _ (z1 :: _) with "[//]").
-    iIntros (v) "[[% %] | (% & % & % & %)]"; [done|]; simplify_eq.
+    wp_apply (wp_list_head _ _ zs1 with "[//]").
+    iIntros (v) "[[-> ->] | (%z1 & %zs1' & -> & ->)]".
+    { wp_pures. rewrite bool_decide_eq_true_2 //. by iApply "H". }
     wp_pures.
-    wp_apply (wp_list_head _ _ (z2 :: _) with "[//]").
-    iIntros (v) "[[% %] | (% & % & % & %)]"; [done|]; simplify_eq.
+    wp_apply (wp_list_head _ _ zs2 with "[//]").
+    iIntros (v) "[[-> ->] | (%z2 & %zs2' & -> & ->)]".
+    { wp_pures. rewrite bool_decide_eq_false_2 /=; auto. by iApply "H". }
     wp_pures.
-    iApply "H".
+    simpl.
     iModIntro.
-    iSplit; by iExists _.
+    iSpecialize ("H" with "[//]").
+    destruct (decide (z1 ≤ z2)%Z).
+    { do 2 (rewrite bool_decide_eq_true_2 //). }
+    do 2 (rewrite bool_decide_eq_false_2 //).
   Qed.
 
 End Z_comparator_spec.
 
-Program Definition Z_loc_comparator : comparator Z CostTick :=
+Program Definition Z_list_comparator : comparator (list Z) CostTick :=
   {| cmp := cmp_Z_list;
-     cmp_rel := Z.le;
+     cmp_rel := list_Z_le;
      cmp_cost := 0%R;
      cmp_has_key _ _ := is_Z_list;
      wp_cmp := _;
@@ -86,7 +99,7 @@ Section kway_merge.
   Definition merge : val :=
     λ: "zss",
       let: "h" := heap_new #() in
-      list_iter (heap_insert "h") "zss";;
+      list_iter (λ: "zs", heap_insert "h" "zs") "zss";;
       let: "out" := ref list_nil in
       repeat_remove "h" "out";;
       list_rev !"out".
@@ -94,24 +107,97 @@ Section kway_merge.
 End kway_merge.
 
 Section kway_merge_spec.
-  Context `{!ert_clutchGS Σ CostTick} `{!min_heap Z_loc_comparator}.
+  Context `{!ert_clutchGS Σ CostTick} `{!min_heap Z_list_comparator}.
+
+  Local Hint Resolve heap_insert_cost_nonneg : core.
+  Local Hint Resolve heap_remove_cost_nonneg : core.
+
+  (** We give a rough bound by requiring, e.g., [len * (heap_insert_cost len)] credits even though,
+      in reality, only
+
+        [heap_insert_cost 0 + heap_insert_cost 1 + ... + heap_insert_cost len]
+
+      should be necessary. *)
+  Definition repeat_remove_cost (zss : list (list Z)) : R :=
+    let len := length zss in
+    let total := sum_list_with length zss in
+    (** A list is removed from the heap for all elements + an extra removal for the empty lists *)
+    (total + len) * heap_remove_cost len +
+    (** A list is inserted for all elements, (except the initial head elements which are inserted as
+        part of [merge] so we should in theory subtract [len] from [total]. *)
+    total * heap_insert_cost len.
 
   Definition merge_cost (zss : list (list Z)) : R :=
     let len := length zss in
-    let total := sum_list_with length zss in
-    (** initial insertion  *)
-    len * heap_insert_cost len +
-    (** loop  *)
-    (total + len) * heap_remove_cost len +
-    total * heap_insert_cost len.
+    len * heap_insert_cost len + repeat_remove_cost zss.
+
+
+  Lemma repeat_remove_cost_nonneg zss :
+    (0 <= repeat_remove_cost zss)%R.
+  Proof.
+    rewrite /repeat_remove_cost.
+  Admitted.
+
+  Local Hint Resolve repeat_remove_cost_nonneg : core.
+
+  Lemma wp_repeat_remove h out (zss : list (list Z)) v :
+    is_list zss v →
+    Forall (Sorted Z.le) zss →
+    {{{ ⧖ (repeat_remove_cost zss) ∗ is_min_heap zss h ∗ out ↦ NONEV }}}
+      repeat_remove h #out
+    {{{ zs v, RET #();
+        is_min_heap [] h ∗ out ↦ inject zs ∗
+        ⌜is_list zs v⌝ ∗ ⌜zs ≡ₚ concat zss⌝ ∗ ⌜Sorted (flip Z.le) zs⌝}}}.
+  Proof.
+    Admitted.
+
 
   Lemma wp_merge (v : val) (zss : list (list Z)) :
     is_list zss v →
-    Forall (λ zs, is_list zs (inject zs) ∧ Sorted Z.le zs) zss →
+    Forall (Sorted Z.le) zss →
     {{{ ⧖ (merge_cost zss) }}}
       merge v
     {{{ v zs, RET v; ⌜is_list zs v⌝ ∗ ⌜zs ≡ₚ concat zss⌝ ∗ ⌜Sorted Z.le zs⌝ }}}.
   Proof.
-    Admitted.
+    iIntros (Hv Hzss Ψ) "Hc HΨ".
+    rewrite /merge_cost.
+    iDestruct (etc_split with "Hc") as "[Hinit Hc]".
+    { assert (0 <= length zss)%R by eauto with real. real_solver. }
+    { auto. }
+    wp_rec.
+    wp_apply wp_heap_new; [done|].
+    iIntros (h) "Hh"; wp_pures.
+    rewrite etc_split_list; [|apply heap_insert_cost_nonneg].
+    wp_apply (wp_list_iter_invariant (λ _, ⧖ (heap_insert_cost (length zss))) (λ _, True)
+                (λ l, is_min_heap l h) True with "[] [$Hh $Hinit //]")%I.
+    { iIntros (l l' Ψ') "!# ([% ->] & _ & Hh & Hc) HΨ'".
+      rewrite app_length /=.
+      (** Here we possibly throw away some credits *)
+      iDestruct (etc_weaken _ (heap_insert_cost (length l')) with "Hc") as "Hc".
+      { split; [auto|]. apply heap_insert_cost_mono. lia. }
+      wp_pures.
+      wp_apply (wp_heap_insert _ l with "[$Hh $Hc]").
+      { rewrite /= /is_Z_list is_list_inject //. }
+      iIntros (zss') "[Hh ->]".
+      iApply "HΨ'".
+      rewrite Permutation_cons_append.
+      iFrame. }
+    iIntros "(_ & Hh & _)".
+    wp_pures.
+    wp_alloc out as "Hout".
+    wp_pures.
+    wp_apply (wp_repeat_remove with "[$Hc $Hh $Hout]"); [done|done|].
+    iIntros (zs w) "(Hh & Hout & %Hzs & %Hp & %Hsorted)".
+    wp_pures.
+    wp_load; iIntros "Hout".
+    wp_apply (wp_list_rev _ _ zs with "[]").
+    { rewrite is_list_inject //. }
+    iIntros (u Hu) .
+    iApply "HΨ".
+    iFrame "%".
+    iSplit; iPureIntro.
+    { rewrite reverse_Permutation //. }
+    by apply Sorted_reverse in Hsorted.
+  Qed.
 
 End kway_merge_spec.
